

Exercise 1.1

Question 11

$$(a) \quad 3x - 2y = 4 \rightarrow (i)$$

$$6x - 4y = 9 \rightarrow (ii)$$

Multiplying equ (i) by -2

$$-6x + 4y = -8 \rightarrow (iii)$$

Adding equ (ii) and (iii)

$$-6x + 4y = -8$$

$$6x - 4y = 9$$

$$0 = 1$$

Hence, the final equations are

$$3x - 2y = 4$$

$$0 = 1$$

Since the second equation is contradictory
so the original system has no solutions.

$$(b) \quad 2x - 4y = 1 \rightarrow (i)$$

$$4x - 8y = 2 \rightarrow (ii)$$

Multiplying equ (i) by -2

$$-4x + 8y = -2 \rightarrow (iii)$$

Adding equ (ii) and (iii)

$$-4x + 8y = -2$$

$$4x - 8y = 2$$

$$\Rightarrow 0 = 0$$

Hence, the final equations are

$$2x - 4y = 1$$

$$0 = 0$$

The second equation does not impose any restriction on x and y therefore we can omit it. Also,

$$2x - 4y = 1$$

$$2x = 4y + 1$$

$$x = 2y + \frac{1}{2}$$

$$\text{or, } x = 2t + \frac{1}{2}, \quad y = t$$

where, t is an arbitrary real number.

$$(c) \quad x - 2y = 0 \rightarrow (i)$$

$$x - 4y = 8 \rightarrow (ii)$$

Subtracting eqn (i) from (ii)

$$x - 4y = 8$$

$$\underline{-x + 2y = 0}$$

$$-2y = 8$$

$$\boxed{y = -4}$$

Putting $y = -4$ in eqn (i)

$$x - 2(-4) = 0$$

$$x + 8 = 0$$

$$\boxed{x = -8}$$

Question 12 :-

$$2x - 3y = a \rightarrow (i)$$

$$4x - 6y = b \rightarrow (ii)$$

Multiplying eqn (i) by -2

$$-4x + 6y = -2a \rightarrow (iii)$$

Adding eqn (ii) and (iii)

$$4x - 6y = b$$

$$-4x + 6y = -2a$$

$$0 = b - 2a$$

Thus, the final equations are

$$2x - 3y = a$$

$$0 = b - 2a$$

\Rightarrow If $b - 2a = 0$ ($b = 2a$) then the system has infinitely many solutions.

\Rightarrow If $b - 2a \neq 0$ ($b \neq 2a$) then the system has no solutions.

\Rightarrow There are no values of a and b for which the system has one solution.

Question 13 :-

$$(c) \quad 3v - 8w + 2x - y + 4z = 0$$

Solving the equation for v , we obtain

$$3v = 8w - 2x + y - 4z$$

$$v = \frac{8}{3}w - \frac{2}{3}x + \frac{1}{3}y - \frac{4}{3}z$$

and,

$$v = \frac{8}{3}t_1 - \frac{2}{3}t_2 + \frac{1}{3}t_3 - \frac{4}{3}t_4$$

$$w = t_1, \quad y = t_3, \quad x = t_2, \quad z = t_4$$

Question 14 :-

(c) $4x_1 + 2x_2 + 3x_3 + x_4 = 20$

Solving the equation for x_1 , we get

$$4x_1 = -2x_2 + 3x_3 - x_4 + 20$$

$$x_1 = -\frac{2}{4}x_2 + \frac{3}{4}x_3 - \frac{1}{4}x_4 + \frac{20}{4}$$

$$x_1 = 5 - \frac{1}{2}x_2 - \frac{3}{4}x_3 - \frac{1}{4}x_4$$

and,

$$x_1 = 5 - \frac{1}{2}s - \frac{3}{4}s - \frac{1}{4}t$$

$$x_2 = s, \quad x_3 = s, \quad x_4 = t$$